tools/generated/compiler_extracted.ml
@@ -1,0 +1,2559 @@
+
+type bool =
+| True
+| False
+
+(** val negb : bool -> bool **)
+
+let negb = function
+| True -> False
+| False -> True
+
+type nat =
+| O
+| S of nat
+
+type 'a option =
+| Some of 'a
+| None
+
+type ('a, 'b) sum =
+| Inl of 'a
+| Inr of 'b
+
+type ('a, 'b) prod =
+| Pair of 'a * 'b
+
+(** val fst : ('a1, 'a2) prod -> 'a1 **)
+
+let fst = function
+| Pair (x, _) -> x
+
+(** val snd : ('a1, 'a2) prod -> 'a2 **)
+
+let snd = function
+| Pair (_, y) -> y
+
+type 'a list =
+| Nil
+| Cons of 'a * 'a list
+
+(** val length : 'a1 list -> nat **)
+
+let rec length = function
+| Nil -> O
+| Cons (_, l') -> S (length l')
+
+(** val app : 'a1 list -> 'a1 list -> 'a1 list **)
+
+let rec app l m =
+  match l with
+  | Nil -> m
+  | Cons (a, l1) -> Cons (a, (app l1 m))
+
+type comparison =
+| Eq
+| Lt
+| Gt
+
+(** val compOpp : comparison -> comparison **)
+
+let compOpp = function
+| Eq -> Eq
+| Lt -> Gt
+| Gt -> Lt
+
+type sumbool =
+| Left
+| Right
+
+module Coq__1 = struct
+ (** val add : nat -> nat -> nat **)
+
+ let rec add n0 m =
+   match n0 with
+   | O -> m
+   | S p -> S (add p m)
+end
+include Coq__1
+
+(** val mul : nat -> nat -> nat **)
+
+let rec mul n0 m =
+  match n0 with
+  | O -> O
+  | S p -> add m (mul p m)
+
+(** val sub : nat -> nat -> nat **)
+
+let rec sub n0 m =
+  match n0 with
+  | O -> n0
+  | S k -> (match m with
+            | O -> n0
+            | S l -> sub k l)
+
+type positive =
+| XI of positive
+| XO of positive
+| XH
+
+type n =
+| N0
+| Npos of positive
+
+type z =
+| Z0
+| Zpos of positive
+| Zneg of positive
+
+module Pos =
+ struct
+  (** val succ : positive -> positive **)
+
+  let rec succ = function
+  | XI p -> XO (succ p)
+  | XO p -> XI p
+  | XH -> XO XH
+
+  (** val add : positive -> positive -> positive **)
+
+  let rec add x y =
+    match x with
+    | XI p ->
+      (match y with
+       | XI q -> XO (add_carry p q)
+       | XO q -> XI (add p q)
+       | XH -> XO (succ p))
+    | XO p ->
+      (match y with
+       | XI q -> XI (add p q)
+       | XO q -> XO (add p q)
+       | XH -> XI p)
+    | XH -> (match y with
+             | XI q -> XO (succ q)
+             | XO q -> XI q
+             | XH -> XO XH)
+
+  (** val add_carry : positive -> positive -> positive **)
+
+  and add_carry x y =
+    match x with
+    | XI p ->
+      (match y with
+       | XI q -> XI (add_carry p q)
+       | XO q -> XO (add_carry p q)
+       | XH -> XI (succ p))
+    | XO p ->
+      (match y with
+       | XI q -> XO (add_carry p q)
+       | XO q -> XI (add p q)
+       | XH -> XO (succ p))
+    | XH ->
+      (match y with
+       | XI q -> XI (succ q)
+       | XO q -> XO (succ q)
+       | XH -> XI XH)
+
+  (** val pred_double : positive -> positive **)
+
+  let rec pred_double = function
+  | XI p -> XI (XO p)
+  | XO p -> XI (pred_double p)
+  | XH -> XH
+
+  (** val pred_N : positive -> n **)
+
+  let pred_N = function
+  | XI p -> Npos (XO p)
+  | XO p -> Npos (pred_double p)
+  | XH -> N0
+
+  type mask =
+  | IsNul
+  | IsPos of positive
+  | IsNeg
+
+  (** val succ_double_mask : mask -> mask **)
+
+  let succ_double_mask = function
+  | IsNul -> IsPos XH
+  | IsPos p -> IsPos (XI p)
+  | IsNeg -> IsNeg
+
+  (** val double_mask : mask -> mask **)
+
+  let double_mask = function
+  | IsPos p -> IsPos (XO p)
+  | x0 -> x0
+
+  (** val double_pred_mask : positive -> mask **)
+
+  let double_pred_mask = function
+  | XI p -> IsPos (XO (XO p))
+  | XO p -> IsPos (XO (pred_double p))
+  | XH -> IsNul
+
+  (** val sub_mask : positive -> positive -> mask **)
+
+  let rec sub_mask x y =
+    match x with
+    | XI p ->
+      (match y with
+       | XI q -> double_mask (sub_mask p q)
+       | XO q -> succ_double_mask (sub_mask p q)
+       | XH -> IsPos (XO p))
+    | XO p ->
+      (match y with
+       | XI q -> succ_double_mask (sub_mask_carry p q)
+       | XO q -> double_mask (sub_mask p q)
+       | XH -> IsPos (pred_double p))
+    | XH -> (match y with
+             | XH -> IsNul
+             | _ -> IsNeg)
+
+  (** val sub_mask_carry : positive -> positive -> mask **)
+
+  and sub_mask_carry x y =
+    match x with
+    | XI p ->
+      (match y with
+       | XI q -> succ_double_mask (sub_mask_carry p q)
+       | XO q -> double_mask (sub_mask p q)
+       | XH -> IsPos (pred_double p))
+    | XO p ->
+      (match y with
+       | XI q -> double_mask (sub_mask_carry p q)
+       | XO q -> succ_double_mask (sub_mask_carry p q)
+       | XH -> double_pred_mask p)
+    | XH -> IsNeg
+
+  (** val mul : positive -> positive -> positive **)
+
+  let rec mul x y =
+    match x with
+    | XI p -> add y (XO (mul p y))
+    | XO p -> XO (mul p y)
+    | XH -> y
+
+  (** val iter : ('a1 -> 'a1) -> 'a1 -> positive -> 'a1 **)
+
+  let rec iter f x = function
+  | XI n' -> f (iter f (iter f x n') n')
+  | XO n' -> iter f (iter f x n') n'
+  | XH -> f x
+
+  (** val div2 : positive -> positive **)
+
+  let div2 = function
+  | XI p0 -> p0
+  | XO p0 -> p0
+  | XH -> XH
+
+  (** val div2_up : positive -> positive **)
+
+  let div2_up = function
+  | XI p0 -> succ p0
+  | XO p0 -> p0
+  | XH -> XH
+
+  (** val compare_cont : comparison -> positive -> positive -> comparison **)
+
+  let rec compare_cont r x y =
+    match x with
+    | XI p ->
+      (match y with
+       | XI q -> compare_cont r p q
+       | XO q -> compare_cont Gt p q
+       | XH -> Gt)
+    | XO p ->
+      (match y with
+       | XI q -> compare_cont Lt p q
+       | XO q -> compare_cont r p q
+       | XH -> Gt)
+    | XH -> (match y with
+             | XH -> r
+             | _ -> Lt)
+
+  (** val compare : positive -> positive -> comparison **)
+
+  let compare =
+    compare_cont Eq
+
+  (** val coq_Nsucc_double : n -> n **)
+
+  let coq_Nsucc_double = function
+  | N0 -> Npos XH
+  | Npos p -> Npos (XI p)
+
+  (** val coq_Ndouble : n -> n **)
+
+  let coq_Ndouble = function
+  | N0 -> N0
+  | Npos p -> Npos (XO p)
+
+  (** val coq_lor : positive -> positive -> positive **)
+
+  let rec coq_lor p q =
+    match p with
+    | XI p0 ->
+      (match q with
+       | XI q0 -> XI (coq_lor p0 q0)
+       | XO q0 -> XI (coq_lor p0 q0)
+       | XH -> p)
+    | XO p0 ->
+      (match q with
+       | XI q0 -> XI (coq_lor p0 q0)
+       | XO q0 -> XO (coq_lor p0 q0)
+       | XH -> XI p0)
+    | XH -> (match q with
+             | XO q0 -> XI q0
+             | _ -> q)
+
+  (** val coq_land : positive -> positive -> n **)
+
+  let rec coq_land p q =
+    match p with
+    | XI p0 ->
+      (match q with
+       | XI q0 -> coq_Nsucc_double (coq_land p0 q0)
+       | XO q0 -> coq_Ndouble (coq_land p0 q0)
+       | XH -> Npos XH)
+    | XO p0 ->
+      (match q with
+       | XI q0 -> coq_Ndouble (coq_land p0 q0)
+       | XO q0 -> coq_Ndouble (coq_land p0 q0)
+       | XH -> N0)
+    | XH -> (match q with
+             | XO _ -> N0
+             | _ -> Npos XH)
+
+  (** val ldiff : positive -> positive -> n **)
+
+  let rec ldiff p q =
+    match p with
+    | XI p0 ->
+      (match q with
+       | XI q0 -> coq_Ndouble (ldiff p0 q0)
+       | XO q0 -> coq_Nsucc_double (ldiff p0 q0)
+       | XH -> Npos (XO p0))
+    | XO p0 ->
+      (match q with
+       | XI q0 -> coq_Ndouble (ldiff p0 q0)
+       | XO q0 -> coq_Ndouble (ldiff p0 q0)
+       | XH -> Npos p)
+    | XH -> (match q with
+             | XO _ -> Npos XH
+             | _ -> N0)
+
+  (** val coq_lxor : positive -> positive -> n **)
+
+  let rec coq_lxor p q =
+    match p with
+    | XI p0 ->
+      (match q with
+       | XI q0 -> coq_Ndouble (coq_lxor p0 q0)
+       | XO q0 -> coq_Nsucc_double (coq_lxor p0 q0)
+       | XH -> Npos (XO p0))
+    | XO p0 ->
+      (match q with
+       | XI q0 -> coq_Nsucc_double (coq_lxor p0 q0)
+       | XO q0 -> coq_Ndouble (coq_lxor p0 q0)
+       | XH -> Npos (XI p0))
+    | XH ->
+      (match q with
+       | XI q0 -> Npos (XO q0)
+       | XO q0 -> Npos (XI q0)
+       | XH -> N0)
+
+  (** val iter_op : ('a1 -> 'a1 -> 'a1) -> positive -> 'a1 -> 'a1 **)
+
+  let rec iter_op op p a =
+    match p with
+    | XI p0 -> op a (iter_op op p0 (op a a))
+    | XO p0 -> iter_op op p0 (op a a)
+    | XH -> a
+
+  (** val to_nat : positive -> nat **)
+
+  let to_nat x =
+    iter_op Coq__1.add x (S O)
+
+  (** val of_succ_nat : nat -> positive **)
+
+  let rec of_succ_nat = function
+  | O -> XH
+  | S x -> succ (of_succ_nat x)
+ end
+
+module Coq_Pos =
+ struct
+  (** val succ : positive -> positive **)
+
+  let rec succ = function
+  | XI p -> XO (succ p)
+  | XO p -> XI p
+  | XH -> XO XH
+
+  (** val pred_double : positive -> positive **)
+
+  let rec pred_double = function
+  | XI p -> XI (XO p)
+  | XO p -> XI (pred_double p)
+  | XH -> XH
+
+  (** val pred_N : positive -> n **)
+
+  let pred_N = function
+  | XI p -> Npos (XO p)
+  | XO p -> Npos (pred_double p)
+  | XH -> N0
+
+  (** val iter : ('a1 -> 'a1) -> 'a1 -> positive -> 'a1 **)
+
+  let rec iter f x = function
+  | XI n' -> f (iter f (iter f x n') n')
+  | XO n' -> iter f (iter f x n') n'
+  | XH -> f x
+
+  (** val of_succ_nat : nat -> positive **)
+
+  let rec of_succ_nat = function
+  | O -> XH
+  | S x -> succ (of_succ_nat x)
+
+  (** val size : positive -> positive **)
+
+  let rec size = function
+  | XI p0 -> succ (size p0)
+  | XO p0 -> succ (size p0)
+  | XH -> XH
+
+  (** val testbit : positive -> n -> bool **)
+
+  let rec testbit p n0 =
+    match p with
+    | XI p0 -> (match n0 with
+                | N0 -> True
+                | Npos n1 -> testbit p0 (pred_N n1))
+    | XO p0 -> (match n0 with
+                | N0 -> False
+                | Npos n1 -> testbit p0 (pred_N n1))
+    | XH -> (match n0 with
+             | N0 -> True
+             | Npos _ -> False)
+
+  (** val eq_dec : positive -> positive -> sumbool **)
+
+  let rec eq_dec p x0 =
+    match p with
+    | XI p0 -> (match x0 with
+                | XI p1 -> eq_dec p0 p1
+                | _ -> Right)
+    | XO p0 -> (match x0 with
+                | XO p1 -> eq_dec p0 p1
+                | _ -> Right)
+    | XH -> (match x0 with
+             | XH -> Left
+             | _ -> Right)
+ end
+
+module N =
+ struct
+  (** val succ_double : n -> n **)
+
+  let succ_double = function
+  | N0 -> Npos XH
+  | Npos p -> Npos (XI p)
+
+  (** val double : n -> n **)
+
+  let double = function
+  | N0 -> N0
+  | Npos p -> Npos (XO p)
+
+  (** val succ_pos : n -> positive **)
+
+  let succ_pos = function
+  | N0 -> XH
+  | Npos p -> Pos.succ p
+
+  (** val sub : n -> n -> n **)
+
+  let sub n0 m =
+    match n0 with
+    | N0 -> N0
+    | Npos n' ->
+      (match m with
+       | N0 -> n0
+       | Npos m' ->
+         (match Pos.sub_mask n' m' with
+          | Pos.IsPos p -> Npos p
+          | _ -> N0))
+
+  (** val compare : n -> n -> comparison **)
+
+  let compare n0 m =
+    match n0 with
+    | N0 -> (match m with
+             | N0 -> Eq
+             | Npos _ -> Lt)
+    | Npos n' -> (match m with
+                  | N0 -> Gt
+                  | Npos m' -> Pos.compare n' m')
+
+  (** val leb : n -> n -> bool **)
+
+  let leb x y =
+    match compare x y with
+    | Gt -> False
+    | _ -> True
+
+  (** val pos_div_eucl : positive -> n -> (n, n) prod **)
+
+  let rec pos_div_eucl a b =
+    match a with
+    | XI a' ->
+      let Pair (q, r) = pos_div_eucl a' b in
+      let r' = succ_double r in
+      (match leb b r' with
+       | True -> Pair ((succ_double q), (sub r' b))
+       | False -> Pair ((double q), r'))
+    | XO a' ->
+      let Pair (q, r) = pos_div_eucl a' b in
+      let r' = double r in
+      (match leb b r' with
+       | True -> Pair ((succ_double q), (sub r' b))
+       | False -> Pair ((double q), r'))
+    | XH ->
+      (match b with
+       | N0 -> Pair (N0, (Npos XH))
+       | Npos p ->
+         (match p with
+          | XH -> Pair ((Npos XH), N0)
+          | _ -> Pair (N0, (Npos XH))))
+
+  (** val coq_lor : n -> n -> n **)
+
+  let coq_lor n0 m =
+    match n0 with
+    | N0 -> m
+    | Npos p -> (match m with
+                 | N0 -> n0
+                 | Npos q -> Npos (Pos.coq_lor p q))
+
+  (** val coq_land : n -> n -> n **)
+
+  let coq_land n0 m =
+    match n0 with
+    | N0 -> N0
+    | Npos p -> (match m with
+                 | N0 -> N0
+                 | Npos q -> Pos.coq_land p q)
+
+  (** val ldiff : n -> n -> n **)
+
+  let ldiff n0 m =
+    match n0 with
+    | N0 -> N0
+    | Npos p -> (match m with
+                 | N0 -> n0
+                 | Npos q -> Pos.ldiff p q)
+
+  (** val coq_lxor : n -> n -> n **)
+
+  let coq_lxor n0 m =
+    match n0 with
+    | N0 -> m
+    | Npos p -> (match m with
+                 | N0 -> n0
+                 | Npos q -> Pos.coq_lxor p q)
+ end
+
+module Coq_N =
+ struct
+  (** val testbit : n -> n -> bool **)
+
+  let testbit a n0 =
+    match a with
+    | N0 -> False
+    | Npos p -> Coq_Pos.testbit p n0
+ end
+
+module Z =
+ struct
+  (** val double : z -> z **)
+
+  let double = function
+  | Z0 -> Z0
+  | Zpos p -> Zpos (XO p)
+  | Zneg p -> Zneg (XO p)
+
+  (** val succ_double : z -> z **)
+
+  let succ_double = function
+  | Z0 -> Zpos XH
+  | Zpos p -> Zpos (XI p)
+  | Zneg p -> Zneg (Pos.pred_double p)
+
+  (** val pred_double : z -> z **)
+
+  let pred_double = function
+  | Z0 -> Zneg XH
+  | Zpos p -> Zpos (Pos.pred_double p)
+  | Zneg p -> Zneg (XI p)
+
+  (** val pos_sub : positive -> positive -> z **)
+
+  let rec pos_sub x y =
+    match x with
+    | XI p ->
+      (match y with
+       | XI q -> double (pos_sub p q)
+       | XO q -> succ_double (pos_sub p q)
+       | XH -> Zpos (XO p))
+    | XO p ->
+      (match y with
+       | XI q -> pred_double (pos_sub p q)
+       | XO q -> double (pos_sub p q)
+       | XH -> Zpos (Pos.pred_double p))
+    | XH ->
+      (match y with
+       | XI q -> Zneg (XO q)
+       | XO q -> Zneg (Pos.pred_double q)
+       | XH -> Z0)
+
+  (** val add : z -> z -> z **)
+
+  let add x y =
+    match x with
+    | Z0 -> y
+    | Zpos x' ->
+      (match y with
+       | Z0 -> x
+       | Zpos y' -> Zpos (Pos.add x' y')
+       | Zneg y' -> pos_sub x' y')
+    | Zneg x' ->
+      (match y with
+       | Z0 -> x
+       | Zpos y' -> pos_sub y' x'
+       | Zneg y' -> Zneg (Pos.add x' y'))
+
+  (** val opp : z -> z **)
+
+  let opp = function
+  | Z0 -> Z0
+  | Zpos x0 -> Zneg x0
+  | Zneg x0 -> Zpos x0
+
+  (** val sub : z -> z -> z **)
+
+  let sub m n0 =
+    add m (opp n0)
+
+  (** val mul : z -> z -> z **)
+
+  let mul x y =
+    match x with
+    | Z0 -> Z0
+    | Zpos x' ->
+      (match y with
+       | Z0 -> Z0
+       | Zpos y' -> Zpos (Pos.mul x' y')
+       | Zneg y' -> Zneg (Pos.mul x' y'))
+    | Zneg x' ->
+      (match y with
+       | Z0 -> Z0
+       | Zpos y' -> Zneg (Pos.mul x' y')
+       | Zneg y' -> Zpos (Pos.mul x' y'))
+
+  (** val compare : z -> z -> comparison **)
+
+  let compare x y =
+    match x with
+    | Z0 -> (match y with
+             | Z0 -> Eq
+             | Zpos _ -> Lt
+             | Zneg _ -> Gt)
+    | Zpos x' -> (match y with
+                  | Zpos y' -> Pos.compare x' y'
+                  | _ -> Gt)
+    | Zneg x' ->
+      (match y with
+       | Zneg y' -> compOpp (Pos.compare x' y')
+       | _ -> Lt)
+
+  (** val leb : z -> z -> bool **)
+
+  let leb x y =
+    match compare x y with
+    | Gt -> False
+    | _ -> True
+
+  (** val ltb : z -> z -> bool **)
+
+  let ltb x y =
+    match compare x y with
+    | Lt -> True
+    | _ -> False
+
+  (** val to_nat : z -> nat **)
+
+  let to_nat = function
+  | Zpos p -> Pos.to_nat p
+  | _ -> O
+
+  (** val of_nat : nat -> z **)
+
+  let of_nat = function
+  | O -> Z0
+  | S n1 -> Zpos (Pos.of_succ_nat n1)
+
+  (** val of_N : n -> z **)
+
+  let of_N = function
+  | N0 -> Z0
+  | Npos p -> Zpos p
+
+  (** val pos_div_eucl : positive -> z -> (z, z) prod **)
+
+  let rec pos_div_eucl a b =
+    match a with
+    | XI a' ->
+      let Pair (q, r) = pos_div_eucl a' b in
+      let r' = add (mul (Zpos (XO XH)) r) (Zpos XH) in
+      (match ltb r' b with
+       | True -> Pair ((mul (Zpos (XO XH)) q), r')
+       | False -> Pair ((add (mul (Zpos (XO XH)) q) (Zpos XH)), (sub r' b)))
+    | XO a' ->
+      let Pair (q, r) = pos_div_eucl a' b in
+      let r' = mul (Zpos (XO XH)) r in
+      (match ltb r' b with
+       | True -> Pair ((mul (Zpos (XO XH)) q), r')
+       | False -> Pair ((add (mul (Zpos (XO XH)) q) (Zpos XH)), (sub r' b)))
+    | XH ->
+      (match leb (Zpos (XO XH)) b with
+       | True -> Pair (Z0, (Zpos XH))
+       | False -> Pair ((Zpos XH), Z0))
+
+  (** val div_eucl : z -> z -> (z, z) prod **)
+
+  let div_eucl a b =
+    match a with
+    | Z0 -> Pair (Z0, Z0)
+    | Zpos a' ->
+      (match b with
+       | Z0 -> Pair (Z0, a)
+       | Zpos _ -> pos_div_eucl a' b
+       | Zneg b' ->
+         let Pair (q, r) = pos_div_eucl a' (Zpos b') in
+         (match r with
+          | Z0 -> Pair ((opp q), Z0)
+          | _ -> Pair ((opp (add q (Zpos XH))), (add b r))))
+    | Zneg a' ->
+      (match b with
+       | Z0 -> Pair (Z0, a)
+       | Zpos _ ->
+         let Pair (q, r) = pos_div_eucl a' b in
+         (match r with
+          | Z0 -> Pair ((opp q), Z0)
+          | _ -> Pair ((opp (add q (Zpos XH))), (sub b r)))
+       | Zneg b' ->
+         let Pair (q, r) = pos_div_eucl a' (Zpos b') in Pair (q, (opp r)))
+
+  (** val div : z -> z -> z **)
+
+  let div a b =
+    let Pair (q, _) = div_eucl a b in q
+
+  (** val modulo : z -> z -> z **)
+
+  let modulo a b =
+    let Pair (_, r) = div_eucl a b in r
+
+  (** val quotrem : z -> z -> (z, z) prod **)
+
+  let quotrem a b =
+    match a with
+    | Z0 -> Pair (Z0, Z0)
+    | Zpos a0 ->
+      (match b with
+       | Z0 -> Pair (Z0, a)
+       | Zpos b0 ->
+         let Pair (q, r) = N.pos_div_eucl a0 (Npos b0) in
+         Pair ((of_N q), (of_N r))
+       | Zneg b0 ->
+         let Pair (q, r) = N.pos_div_eucl a0 (Npos b0) in
+         Pair ((opp (of_N q)), (of_N r)))
+    | Zneg a0 ->
+      (match b with
+       | Z0 -> Pair (Z0, a)
+       | Zpos b0 ->
+         let Pair (q, r) = N.pos_div_eucl a0 (Npos b0) in
+         Pair ((opp (of_N q)), (opp (of_N r)))
+       | Zneg b0 ->
+         let Pair (q, r) = N.pos_div_eucl a0 (Npos b0) in
+         Pair ((of_N q), (opp (of_N r))))
+
+  (** val quot : z -> z -> z **)
+
+  let quot a b =
+    fst (quotrem a b)
+
+  (** val rem : z -> z -> z **)
+
+  let rem a b =
+    snd (quotrem a b)
+
+  (** val div2 : z -> z **)
+
+  let div2 = function
+  | Z0 -> Z0
+  | Zpos p -> (match p with
+               | XH -> Z0
+               | _ -> Zpos (Pos.div2 p))
+  | Zneg p -> Zneg (Pos.div2_up p)
+
+  (** val shiftl : z -> z -> z **)
+
+  let shiftl a = function
+  | Z0 -> a
+  | Zpos p -> Pos.iter (mul (Zpos (XO XH))) a p
+  | Zneg p -> Pos.iter div2 a p
+
+  (** val shiftr : z -> z -> z **)
+
+  let shiftr a n0 =
+    shiftl a (opp n0)
+
+  (** val coq_lor : z -> z -> z **)
+
+  let coq_lor a b =
+    match a with
+    | Z0 -> b
+    | Zpos a0 ->
+      (match b with
+       | Z0 -> a
+       | Zpos b0 -> Zpos (Pos.coq_lor a0 b0)
+       | Zneg b0 -> Zneg (N.succ_pos (N.ldiff (Pos.pred_N b0) (Npos a0))))
+    | Zneg a0 ->
+      (match b with
+       | Z0 -> a
+       | Zpos b0 -> Zneg (N.succ_pos (N.ldiff (Pos.pred_N a0) (Npos b0)))
+       | Zneg b0 ->
+         Zneg (N.succ_pos (N.coq_land (Pos.pred_N a0) (Pos.pred_N b0))))
+
+  (** val coq_land : z -> z -> z **)
+
+  let coq_land a b =
+    match a with
+    | Z0 -> Z0
+    | Zpos a0 ->
+      (match b with
+       | Z0 -> Z0
+       | Zpos b0 -> of_N (Pos.coq_land a0 b0)
+       | Zneg b0 -> of_N (N.ldiff (Npos a0) (Pos.pred_N b0)))
+    | Zneg a0 ->
+      (match b with
+       | Z0 -> Z0
+       | Zpos b0 -> of_N (N.ldiff (Npos b0) (Pos.pred_N a0))
+       | Zneg b0 ->
+         Zneg (N.succ_pos (N.coq_lor (Pos.pred_N a0) (Pos.pred_N b0))))
+
+  (** val coq_lxor : z -> z -> z **)
+
+  let coq_lxor a b =
+    match a with
+    | Z0 -> b
+    | Zpos a0 ->
+      (match b with
+       | Z0 -> a
+       | Zpos b0 -> of_N (Pos.coq_lxor a0 b0)
+       | Zneg b0 -> Zneg (N.succ_pos (N.coq_lxor (Npos a0) (Pos.pred_N b0))))
+    | Zneg a0 ->
+      (match b with
+       | Z0 -> a
+       | Zpos b0 -> Zneg (N.succ_pos (N.coq_lxor (Pos.pred_N a0) (Npos b0)))
+       | Zneg b0 -> of_N (N.coq_lxor (Pos.pred_N a0) (Pos.pred_N b0)))
+
+  (** val pred : z -> z **)
+
+  let pred x =
+    add x (Zneg XH)
+
+  (** val iter : z -> ('a1 -> 'a1) -> 'a1 -> 'a1 **)
+
+  let iter n0 f x =
+    match n0 with
+    | Zpos p -> Coq_Pos.iter f x p
+    | _ -> x
+
+  (** val odd : z -> bool **)
+
+  let odd = function
+  | Z0 -> False
+  | Zpos p -> (match p with
+               | XO _ -> False
+               | _ -> True)
+  | Zneg p -> (match p with
+               | XO _ -> False
+               | _ -> True)
+
+  (** val log2 : z -> z **)
+
+  let log2 = function
+  | Zpos p0 ->
+    (match p0 with
+     | XI p -> Zpos (Coq_Pos.size p)
+     | XO p -> Zpos (Coq_Pos.size p)
+     | XH -> Z0)
+  | _ -> Z0
+
+  (** val testbit : z -> z -> bool **)
+
+  let testbit a = function
+  | Z0 -> odd a
+  | Zpos p ->
+    (match a with
+     | Z0 -> False
+     | Zpos a0 -> Coq_Pos.testbit a0 (Npos p)
+     | Zneg a0 -> negb (Coq_N.testbit (Coq_Pos.pred_N a0) (Npos p)))
+  | Zneg _ -> False
+
+  (** val eq_dec : z -> z -> sumbool **)
+
+  let eq_dec x y =
+    match x with
+    | Z0 -> (match y with
+             | Z0 -> Left
+             | _ -> Right)
+    | Zpos p -> (match y with
+                 | Zpos p0 -> Coq_Pos.eq_dec p p0
+                 | _ -> Right)
+    | Zneg p -> (match y with
+                 | Zneg p0 -> Coq_Pos.eq_dec p p0
+                 | _ -> Right)
+
+  (** val ones : z -> z **)
+
+  let ones n0 =
+    pred (shiftl (Zpos XH) n0)
+ end
+
+(** val z_lt_dec : z -> z -> sumbool **)
+
+let z_lt_dec x y =
+  match Z.compare x y with
+  | Lt -> Left
+  | _ -> Right
+
+(** val z_le_dec : z -> z -> sumbool **)
+
+let z_le_dec x y =
+  match Z.compare x y with
+  | Gt -> Right
+  | _ -> Left
+
+(** val z_le_gt_dec : z -> z -> sumbool **)
+
+let z_le_gt_dec =
+  z_le_dec
+
+(** val map : ('a1 -> 'a2) -> 'a1 list -> 'a2 list **)
+
+let rec map f = function
+| Nil -> Nil
+| Cons (a, l0) -> Cons ((f a), (map f l0))
+
+(** val seq : nat -> nat -> nat list **)
+
+let rec seq start = function
+| O -> Nil
+| S len0 -> Cons (start, (seq (S start) len0))
+
+(** val fold_right : ('a2 -> 'a1 -> 'a1) -> 'a1 -> 'a2 list -> 'a1 **)
+
+let rec fold_right f a0 = function
+| Nil -> a0
+| Cons (b, l0) -> f b (fold_right f a0 l0)
+
+(** val shift_nat : nat -> positive -> positive **)
+
+let rec shift_nat n0 z0 =
+  match n0 with
+  | O -> z0
+  | S n1 -> XO (shift_nat n1 z0)
+
+(** val shift_pos : positive -> positive -> positive **)
+
+let shift_pos n0 z0 =
+  Coq_Pos.iter (fun x -> XO x) z0 n0
+
+(** val two_power_nat : nat -> z **)
+
+let two_power_nat n0 =
+  Zpos (shift_nat n0 XH)
+
+(** val two_power_pos : positive -> z **)
+
+let two_power_pos x =
+  Zpos (shift_pos x XH)
+
+(** val two_p : z -> z **)
+
+let two_p = function
+| Z0 -> Zpos XH
+| Zpos y -> two_power_pos y
+| Zneg _ -> Z0
+
+module Byte =
+ struct
+  type t = z
+    (* singleton inductive, whose constructor was Build_t *)
+
+  (** val unsigned : t -> z **)
+
+  let unsigned t0 =
+    t0
+ end
+
+(** val byte_nat : Byte.t -> nat **)
+
+let byte_nat =
+  Z.to_nat
+
+type opcode =
+| OpStop
+| OpLoad of nat
+| OpStore of nat
+| OpPop
+| OpAdd
+| OpSub
+| OpDup
+| OpJumpdest
+| OpJumpi
+
+(** val opcode_width : opcode -> nat **)
+
+let opcode_width = function
+| OpLoad _ -> S (S O)
+| OpStore _ -> S (S O)
+| _ -> S O
+
+type instruction = { instr_pc : nat; instr_opcode : opcode; instr_next : nat }
+
+(** val make_instruction : nat -> opcode -> instruction **)
+
+let make_instruction pc op =
+  { instr_pc = pc; instr_opcode = op; instr_next =
+    (add pc (opcode_width op)) }
+
+type parse_error =
+| UnknownOpcode of nat * nat
+| TruncatedOperand of nat
+
+type 'a parse_result =
+| Parsed of 'a
+| Rejected of parse_error
+
+(** val prepend_instruction :
+    instruction -> instruction list parse_result -> instruction list
+    parse_result **)
+
+let prepend_instruction i = function
+| Parsed code0 -> Parsed (Cons (i, code0))
+| Rejected error -> Rejected error
+
+type operand_kind =
+| LoadOperand
+| StoreOperand
+
+type scan_mode =
+| ExpectOpcode of nat
+| ExpectOperand of nat * operand_kind
+
+(** val scan : scan_mode -> Byte.t list -> instruction list parse_result **)
+
+let rec scan mode bytes =
+  match mode with
+  | ExpectOpcode pc ->
+    (match bytes with
+     | Nil -> Parsed Nil
+     | Cons (opbyte, tail) ->
+       (match byte_nat opbyte with
+        | O ->
+          prepend_instruction (make_instruction pc OpStop)
+            (scan (ExpectOpcode (S pc)) tail)
+        | S n0 ->
+          (match n0 with
+           | O -> scan (ExpectOperand (pc, LoadOperand)) tail
+           | S n1 ->
+             (match n1 with
+              | O -> scan (ExpectOperand (pc, StoreOperand)) tail
+              | S n2 ->
+                (match n2 with
+                 | O ->
+                   prepend_instruction (make_instruction pc OpPop)
+                     (scan (ExpectOpcode (S pc)) tail)
+                 | S n3 ->
+                   (match n3 with
+                    | O ->
+                      prepend_instruction (make_instruction pc OpAdd)
+                        (scan (ExpectOpcode (S pc)) tail)
+                    | S n4 ->
+                      (match n4 with
+                       | O ->
+                         prepend_instruction (make_instruction pc OpSub)
+                           (scan (ExpectOpcode (S pc)) tail)
+                       | S n5 ->
+                         (match n5 with
+                          | O ->
+                            prepend_instruction (make_instruction pc OpDup)
+                              (scan (ExpectOpcode (S pc)) tail)
+                          | S n6 ->
+                            (match n6 with
+                             | O ->
+                               prepend_instruction
+                                 (make_instruction pc OpJumpdest)
+                                 (scan (ExpectOpcode (S pc)) tail)
+                             | S n7 ->
+                               (match n7 with
+                                | O ->
+                                  prepend_instruction
+                                    (make_instruction pc OpJumpi)
+                                    (scan (ExpectOpcode (S pc)) tail)
+                                | S n8 ->
+                                  Rejected (UnknownOpcode (pc, (S (S (S (S (S
+                                    (S (S (S (S n8)))))))))))))))))))))
+  | ExpectOperand (pc, kind) ->
+    (match kind with
+     | LoadOperand ->
+       (match bytes with
+        | Nil -> Rejected (TruncatedOperand pc)
+        | Cons (operand, tail) ->
+          prepend_instruction
+            (make_instruction pc (OpLoad (byte_nat operand)))
+            (scan (ExpectOpcode (add pc (S (S O)))) tail))
+     | StoreOperand ->
+       (match bytes with
+        | Nil -> Rejected (TruncatedOperand pc)
+        | Cons (operand, tail) ->
+          prepend_instruction
+            (make_instruction pc (OpStore (byte_nat operand)))
+            (scan (ExpectOpcode (add pc (S (S O)))) tail)))
+
+type program = { program_bytes : Byte.t list; program_code : instruction list }
+
+(** val parse : Byte.t list -> program parse_result **)
+
+let parse bytes =
+  match scan (ExpectOpcode O) bytes with
+  | Parsed code0 -> Parsed { program_bytes = bytes; program_code = code0 }
+  | Rejected error -> Rejected error
+
+type ascii =
+| Ascii of bool * bool * bool * bool * bool * bool * bool * bool
+
+type string =
+| EmptyString
+| String of ascii * string
+
+(** val zeq : z -> z -> sumbool **)
+
+let zeq =
+  Z.eq_dec
+
+(** val zlt : z -> z -> sumbool **)
+
+let zlt =
+  z_lt_dec
+
+(** val zle : z -> z -> sumbool **)
+
+let zle =
+  z_le_gt_dec
+
+(** val proj_sumbool : sumbool -> bool **)
+
+let proj_sumbool = function
+| Left -> True
+| Right -> False
+
+(** val p_mod_two_p : positive -> nat -> z **)
+
+let rec p_mod_two_p p = function
+| O -> Z0
+| S m ->
+  (match p with
+   | XI q -> Z.succ_double (p_mod_two_p q m)
+   | XO q -> Z.double (p_mod_two_p q m)
+   | XH -> Zpos XH)
+
+(** val zshiftin : bool -> z -> z **)
+
+let zshiftin b x =
+  match b with
+  | True -> Z.succ_double x
+  | False -> Z.double x
+
+(** val zzero_ext : z -> z -> z **)
+
+let zzero_ext n0 x =
+  Z.iter n0 (fun rec0 x0 -> zshiftin (Z.odd x0) (rec0 (Z.div2 x0))) (fun _ ->
+    Z0) x
+
+(** val zsign_ext : z -> z -> z **)
+
+let zsign_ext n0 x =
+  Z.iter (Z.pred n0) (fun rec0 x0 -> zshiftin (Z.odd x0) (rec0 (Z.div2 x0)))
+    (fun x0 ->
+    match match Z.odd x0 with
+          | True -> proj_sumbool (zlt Z0 n0)
+          | False -> False with
+    | True -> Zneg XH
+    | False -> Z0) x
+
+(** val z_one_bits : nat -> z -> z -> z list **)
+
+let rec z_one_bits n0 x i =
+  match n0 with
+  | O -> Nil
+  | S m ->
+    (match Z.odd x with
+     | True -> Cons (i, (z_one_bits m (Z.div2 x) (Z.add i (Zpos XH))))
+     | False -> z_one_bits m (Z.div2 x) (Z.add i (Zpos XH)))
+
+(** val p_is_power2 : positive -> bool **)
+
+let rec p_is_power2 = function
+| XI _ -> False
+| XO q -> p_is_power2 q
+| XH -> True
+
+(** val z_is_power2 : z -> z option **)
+
+let z_is_power2 x = match x with
+| Zpos p -> (match p_is_power2 p with
+             | True -> Some (Z.log2 x)
+             | False -> None)
+| _ -> None
+
+(** val zsize : z -> z **)
+
+let zsize = function
+| Zpos p -> Zpos (Coq_Pos.size p)
+| _ -> Z0
+
+type binary_float =
+| B754_zero of bool
+| B754_infinity of bool
+| B754_nan of bool * positive
+| B754_finite of bool * positive * z
+
+type binary32 = binary_float
+
+type binary64 = binary_float
+
+(** val ptr64 : bool **)
+
+let ptr64 =
+  True
+
+type comparison0 =
+| Ceq
+| Cne
+| Clt
+| Cle
+| Cgt
+| Cge
+
+module type WORDSIZE =
+ sig
+  val wordsize : nat
+ end
+
+module Make =
+ functor (WS:WORDSIZE) ->
+ struct
+  (** val wordsize : nat **)
+
+  let wordsize =
+    WS.wordsize
+
+  (** val zwordsize : z **)
+
+  let zwordsize =
+    Z.of_nat wordsize
+
+  (** val modulus : z **)
+
+  let modulus =
+    two_power_nat wordsize
+
+  (** val half_modulus : z **)
+
+  let half_modulus =
+    Z.div modulus (Zpos (XO XH))
+
+  (** val max_unsigned : z **)
+
+  let max_unsigned =
+    Z.sub modulus (Zpos XH)
+
+  (** val max_signed : z **)
+
+  let max_signed =
+    Z.sub half_modulus (Zpos XH)
+
+  (** val min_signed : z **)
+
+  let min_signed =
+    Z.opp half_modulus
+
+  type int = z
+    (* singleton inductive, whose constructor was mkint *)
+
+  (** val intval : int -> z **)
+
+  let intval i =
+    i
+
+  (** val coq_Z_mod_modulus : z -> z **)
+
+  let coq_Z_mod_modulus = function
+  | Z0 -> Z0
+  | Zpos p -> p_mod_two_p p wordsize
+  | Zneg p ->
+    let r = p_mod_two_p p wordsize in
+    (match zeq r Z0 with
+     | Left -> Z0
+     | Right -> Z.sub modulus r)
+
+  (** val unsigned : int -> z **)
+
+  let unsigned n0 =
+    n0
+
+  (** val signed : int -> z **)
+
+  let signed n0 =
+    let x = unsigned n0 in
+    (match zlt x half_modulus with
+     | Left -> x
+     | Right -> Z.sub x modulus)
+
+  (** val repr : z -> int **)
+
+  let repr =
+    coq_Z_mod_modulus
+
+  (** val zero : int **)
+
+  let zero =
+    repr Z0
+
+  (** val one : int **)
+
+  let one =
+    repr (Zpos XH)
+
+  (** val mone : int **)
+
+  let mone =
+    repr (Zneg XH)
+
+  (** val iwordsize : int **)
+
+  let iwordsize =
+    repr zwordsize
+
+  (** val eq_dec : int -> int -> sumbool **)
+
+  let eq_dec =
+    zeq
+
+  (** val eq : int -> int -> bool **)
+
+  let eq x y =
+    match zeq (unsigned x) (unsigned y) with
+    | Left -> True
+    | Right -> False
+
+  (** val lt : int -> int -> bool **)
+
+  let lt x y =
+    match zlt (signed x) (signed y) with
+    | Left -> True
+    | Right -> False
+
+  (** val ltu : int -> int -> bool **)
+
+  let ltu x y =
+    match zlt (unsigned x) (unsigned y) with
+    | Left -> True
+    | Right -> False
+
+  (** val neg : int -> int **)
+
+  let neg x =
+    repr (Z.opp (unsigned x))
+
+  (** val add : int -> int -> int **)
+
+  let add x y =
+    repr (Z.add (unsigned x) (unsigned y))
+
+  (** val sub : int -> int -> int **)
+
+  let sub x y =
+    repr (Z.sub (unsigned x) (unsigned y))
+
+  (** val mul : int -> int -> int **)
+
+  let mul x y =
+    repr (Z.mul (unsigned x) (unsigned y))
+
+  (** val divs : int -> int -> int **)
+
+  let divs x y =
+    repr (Z.quot (signed x) (signed y))
+
+  (** val mods : int -> int -> int **)
+
+  let mods x y =
+    repr (Z.rem (signed x) (signed y))
+
+  (** val divu : int -> int -> int **)
+
+  let divu x y =
+    repr (Z.div (unsigned x) (unsigned y))
+
+  (** val modu : int -> int -> int **)
+
+  let modu x y =
+    repr (Z.modulo (unsigned x) (unsigned y))
+
+  (** val coq_and : int -> int -> int **)
+
+  let coq_and x y =
+    repr (Z.coq_land (unsigned x) (unsigned y))
+
+  (** val coq_or : int -> int -> int **)
+
+  let coq_or x y =
+    repr (Z.coq_lor (unsigned x) (unsigned y))
+
+  (** val xor : int -> int -> int **)
+
+  let xor x y =
+    repr (Z.coq_lxor (unsigned x) (unsigned y))
+
+  (** val not : int -> int **)
+
+  let not x =
+    xor x mone
+
+  (** val shl : int -> int -> int **)
+
+  let shl x y =
+    repr (Z.shiftl (unsigned x) (unsigned y))
+
+  (** val shru : int -> int -> int **)
+
+  let shru x y =
+    repr (Z.shiftr (unsigned x) (unsigned y))
+
+  (** val shr : int -> int -> int **)
+
+  let shr x y =
+    repr (Z.shiftr (signed x) (unsigned y))
+
+  (** val rol : int -> int -> int **)
+
+  let rol x y =
+    let n0 = Z.modulo (unsigned y) zwordsize in
+    repr
+      (Z.coq_lor (Z.shiftl (unsigned x) n0)
+        (Z.shiftr (unsigned x) (Z.sub zwordsize n0)))
+
+  (** val ror : int -> int -> int **)
+
+  let ror x y =
+    let n0 = Z.modulo (unsigned y) zwordsize in
+    repr
+      (Z.coq_lor (Z.shiftr (unsigned x) n0)
+        (Z.shiftl (unsigned x) (Z.sub zwordsize n0)))
+
+  (** val rolm : int -> int -> int -> int **)
+
+  let rolm x a m =
+    coq_and (rol x a) m
+
+  (** val shrx : int -> int -> int **)
+
+  let shrx x y =
+    divs x (shl one y)
+
+  (** val mulhu : int -> int -> int **)
+
+  let mulhu x y =
+    repr (Z.div (Z.mul (unsigned x) (unsigned y)) modulus)
+
+  (** val mulhs : int -> int -> int **)
+
+  let mulhs x y =
+    repr (Z.div (Z.mul (signed x) (signed y)) modulus)
+
+  (** val negative : int -> int **)
+
+  let negative x =
+    match lt x zero with
+    | True -> one
+    | False -> zero
+
+  (** val add_carry : int -> int -> int -> int **)
+
+  let add_carry x y cin =
+    match zlt (Z.add (Z.add (unsigned x) (unsigned y)) (unsigned cin)) modulus with
+    | Left -> zero
+    | Right -> one
+
+  (** val add_overflow : int -> int -> int -> int **)
+
+  let add_overflow x y cin =
+    let s = Z.add (Z.add (signed x) (signed y)) (signed cin) in
+    (match match proj_sumbool (zle min_signed s) with
+           | True -> proj_sumbool (zle s max_signed)
+           | False -> False with
+     | True -> zero
+     | False -> one)
+
+  (** val sub_borrow : int -> int -> int -> int **)
+
+  let sub_borrow x y bin =
+    match zlt (Z.sub (Z.sub (unsigned x) (unsigned y)) (unsigned bin)) Z0 with
+    | Left -> one
+    | Right -> zero
+
+  (** val sub_overflow : int -> int -> int -> int **)
+
+  let sub_overflow x y bin =
+    let s = Z.sub (Z.sub (signed x) (signed y)) (signed bin) in
+    (match match proj_sumbool (zle min_signed s) with
+           | True -> proj_sumbool (zle s max_signed)
+           | False -> False with
+     | True -> zero
+     | False -> one)
+
+  (** val shr_carry : int -> int -> int **)
+
+  let shr_carry x y =
+    match match lt x zero with
+          | True -> negb (eq (coq_and x (sub (shl one y) one)) zero)
+          | False -> False with
+    | True -> one
+    | False -> zero
+
+  (** val zero_ext : z -> int -> int **)
+
+  let zero_ext n0 x =
+    repr (zzero_ext n0 (unsigned x))
+
+  (** val sign_ext : z -> int -> int **)
+
+  let sign_ext n0 x =
+    repr (zsign_ext n0 (unsigned x))
+
+  (** val one_bits : int -> int list **)
+
+  let one_bits x =
+    map repr (z_one_bits wordsize (unsigned x) Z0)
+
+  (** val is_power2 : int -> int option **)
+
+  let is_power2 x =
+    match z_is_power2 (unsigned x) with
+    | Some i -> Some (repr i)
+    | None -> None
+
+  (** val cmp : comparison0 -> int -> int -> bool **)
+
+  let cmp c x y =
+    match c with
+    | Ceq -> eq x y
+    | Cne -> negb (eq x y)
+    | Clt -> lt x y
+    | Cle -> negb (lt y x)
+    | Cgt -> lt y x
+    | Cge -> negb (lt x y)
+
+  (** val cmpu : comparison0 -> int -> int -> bool **)
+
+  let cmpu c x y =
+    match c with
+    | Ceq -> eq x y
+    | Cne -> negb (eq x y)
+    | Clt -> ltu x y
+    | Cle -> negb (ltu y x)
+    | Cgt -> ltu y x
+    | Cge -> negb (ltu x y)
+
+  (** val notbool : int -> int **)
+
+  let notbool x =
+    match eq x zero with
+    | True -> one
+    | False -> zero
+
+  (** val divmodu2 : int -> int -> int -> (int, int) prod option **)
+
+  let divmodu2 nhi nlo d =
+    match eq_dec d zero with
+    | Left -> None
+    | Right ->
+      let Pair (q, r) =
+        Z.div_eucl (Z.add (Z.mul (unsigned nhi) modulus) (unsigned nlo))
+          (unsigned d)
+      in
+      (match zle q max_unsigned with
+       | Left -> Some (Pair ((repr q), (repr r)))
+       | Right -> None)
+
+  (** val divmods2 : int -> int -> int -> (int, int) prod option **)
+
+  let divmods2 nhi nlo d =
+    match eq_dec d zero with
+    | Left -> None
+    | Right ->
+      let Pair (q, r) =
+        Z.quotrem (Z.add (Z.mul (signed nhi) modulus) (unsigned nlo))
+          (signed d)
+      in
+      (match match proj_sumbool (zle min_signed q) with
+             | True -> proj_sumbool (zle q max_signed)
+             | False -> False with
+       | True -> Some (Pair ((repr q), (repr r)))
+       | False -> None)
+
+  (** val testbit : int -> z -> bool **)
+
+  let testbit x i =
+    Z.testbit (unsigned x) i
+
+  (** val int_of_one_bits : int list -> int **)
+
+  let rec int_of_one_bits = function
+  | Nil -> zero
+  | Cons (a, b) -> add (shl one a) (int_of_one_bits b)
+
+  (** val no_overlap : int -> z -> int -> z -> bool **)
+
+  let no_overlap ofs1 sz1 ofs2 sz2 =
+    let x1 = unsigned ofs1 in
+    let x2 = unsigned ofs2 in
+    (match match proj_sumbool (zlt (Z.add x1 sz1) modulus) with
+           | True -> proj_sumbool (zlt (Z.add x2 sz2) modulus)
+           | False -> False with
+     | True ->
+       (match proj_sumbool (zle (Z.add x1 sz1) x2) with
+        | True -> True
+        | False -> proj_sumbool (zle (Z.add x2 sz2) x1))
+     | False -> False)
+
+  (** val size : int -> z **)
+
+  let size x =
+    zsize (unsigned x)
+
+  (** val unsigned_bitfield_extract : z -> z -> int -> int **)
+
+  let unsigned_bitfield_extract pos width n0 =
+    zero_ext width (shru n0 (repr pos))
+
+  (** val signed_bitfield_extract : z -> z -> int -> int **)
+
+  let signed_bitfield_extract pos width n0 =
+    sign_ext width (shru n0 (repr pos))
+
+  (** val bitfield_insert : z -> z -> int -> int -> int **)
+
+  let bitfield_insert pos width n0 p =
+    let mask0 = shl (repr (Z.sub (two_p width) (Zpos XH))) (repr pos) in
+    coq_or (shl (zero_ext width p) (repr pos)) (coq_and n0 (not mask0))
+ end
+
+module Wordsize_32 =
+ struct
+  (** val wordsize : nat **)
+
+  let wordsize =
+    S (S (S (S (S (S (S (S (S (S (S (S (S (S (S (S (S (S (S (S (S (S (S (S (S
+      (S (S (S (S (S (S (S O)))))))))))))))))))))))))))))))
+ end
+
+module Int = Make(Wordsize_32)
+
+module Wordsize_64 =
+ struct
+  (** val wordsize : nat **)
+
+  let wordsize =
+    S (S (S (S (S (S (S (S (S (S (S (S (S (S (S (S (S (S (S (S (S (S (S (S (S
+      (S (S (S (S (S (S (S (S (S (S (S (S (S (S (S (S (S (S (S (S (S (S (S (S
+      (S (S (S (S (S (S (S (S (S (S (S (S (S (S (S
+      O)))))))))))))))))))))))))))))))))))))))))))))))))))))))))))))))
+ end
+
+module Int64 =
+ struct
+  (** val wordsize : nat **)
+
+  let wordsize =
+    Wordsize_64.wordsize
+
+  (** val modulus : z **)
+
+  let modulus =
+    two_power_nat wordsize
+
+  type int = z
+    (* singleton inductive, whose constructor was mkint *)
+
+  (** val coq_Z_mod_modulus : z -> z **)
+
+  let coq_Z_mod_modulus = function
+  | Z0 -> Z0
+  | Zpos p -> p_mod_two_p p wordsize
+  | Zneg p ->
+    let r = p_mod_two_p p wordsize in
+    (match zeq r Z0 with
+     | Left -> Z0
+     | Right -> Z.sub modulus r)
+
+  (** val repr : z -> int **)
+
+  let repr =
+    coq_Z_mod_modulus
+ end
+
+module Wordsize_Ptrofs =
+ struct
+  (** val wordsize : nat **)
+
+  let wordsize =
+    match ptr64 with
+    | True ->
+      S (S (S (S (S (S (S (S (S (S (S (S (S (S (S (S (S (S (S (S (S (S (S (S
+        (S (S (S (S (S (S (S (S (S (S (S (S (S (S (S (S (S (S (S (S (S (S (S
+        (S (S (S (S (S (S (S (S (S (S (S (S (S (S (S (S (S
+        O)))))))))))))))))))))))))))))))))))))))))))))))))))))))))))))))
+    | False ->
+      S (S (S (S (S (S (S (S (S (S (S (S (S (S (S (S (S (S (S (S (S (S (S (S
+        (S (S (S (S (S (S (S (S O)))))))))))))))))))))))))))))))
+ end
+
+module Ptrofs =
+ struct
+  (** val wordsize : nat **)
+
+  let wordsize =
+    Wordsize_Ptrofs.wordsize
+
+  (** val modulus : z **)
+
+  let modulus =
+    two_power_nat wordsize
+
+  type int = z
+    (* singleton inductive, whose constructor was mkint *)
+
+  (** val coq_Z_mod_modulus : z -> z **)
+
+  let coq_Z_mod_modulus = function
+  | Z0 -> Z0
+  | Zpos p -> p_mod_two_p p wordsize
+  | Zneg p ->
+    let r = p_mod_two_p p wordsize in
+    (match zeq r Z0 with
+     | Left -> Z0
+     | Right -> Z.sub modulus r)
+
+  (** val repr : z -> int **)
+
+  let repr =
+    coq_Z_mod_modulus
+ end
+
+type float = binary64
+
+type float32 = binary32
+
+type ident = positive
+
+type typ =
+| Tint
+| Tfloat
+| Tlong
+| Tsingle
+| Tany32
+| Tany64
+
+type xtype =
+| Xbool
+| Xint8signed
+| Xint8unsigned
+| Xint16signed
+| Xint16unsigned
+| Xint
+| Xfloat
+| Xlong
+| Xsingle
+| Xptr
+| Xany32
+| Xany64
+| Xvoid
+
+type calling_convention = { cc_vararg : z option; cc_unproto : bool;
+                            cc_structret : bool }
+
+(** val cc_default : calling_convention **)
+
+let cc_default =
+  { cc_vararg = None; cc_unproto = False; cc_structret = False }
+
+type signature = { sig_args : xtype list; sig_res : xtype;
+                   sig_cc : calling_convention }
+
+type memory_chunk =
+| Mbool
+| Mint8signed
+| Mint8unsigned
+| Mint16signed
+| Mint16unsigned
+| Mint32
+| Mint64
+| Mfloat32
+| Mfloat64
+| Many32
+| Many64
+
+type external_function =
+| EF_external of string * signature
+| EF_builtin of string * signature
+| EF_runtime of string * signature
+| EF_vload of memory_chunk
+| EF_vstore of memory_chunk
+| EF_malloc
+| EF_free
+| EF_memcpy of z * z
+| EF_annot of positive * string * typ list
+| EF_annot_val of positive * string * typ
+| EF_inline_asm of string * signature * string list
+| EF_debug of positive * ident * typ list
+
+type 'a builtin_arg =
+| BA of 'a
+| BA_int of Int.int
+| BA_long of Int64.int
+| BA_float of float
+| BA_single of float32
+| BA_loadstack of memory_chunk * Ptrofs.int
+| BA_addrstack of Ptrofs.int
+| BA_loadglobal of memory_chunk * ident * Ptrofs.int
+| BA_addrglobal of ident * Ptrofs.int
+| BA_splitlong of 'a builtin_arg * 'a builtin_arg
+| BA_addptr of 'a builtin_arg * 'a builtin_arg
+
+type 'a builtin_res =
+| BR of 'a
+| BR_none
+| BR_splitlong of 'a builtin_res * 'a builtin_res
+
+type ireg =
+| RAX
+| RBX
+| RCX
+| RDX
+| RSI
+| RDI
+| RBP
+| RSP
+| R8
+| R9
+| R10
+| R11
+| R12
+| R13
+| R14
+| R15
+
+type freg =
+| XMM0
+| XMM1
+| XMM2
+| XMM3
+| XMM4
+| XMM5
+| XMM6
+| XMM7
+| XMM8
+| XMM9
+| XMM10
+| XMM11
+| XMM12
+| XMM13
+| XMM14
+| XMM15
+
+type crbit =
+| ZF
+| CF
+| PF
+| SF
+| OF
+
+type preg =
+| PC
+| IR of ireg
+| FR of freg
+| ST0
+| CR of crbit
+| RA
+
+type label = positive
+
+type addrmode =
+| Addrmode of ireg option * (ireg, z) prod option
+   * (z, (ident, Ptrofs.int) prod) sum
+
+type testcond =
+| Cond_e
+| Cond_ne
+| Cond_b
+| Cond_be
+| Cond_ae
+| Cond_a
+| Cond_l
+| Cond_le
+| Cond_ge
+| Cond_g
+| Cond_p
+| Cond_np
+
+type instruction0 =
+| Pmov_rr of ireg * ireg
+| Pmovl_ri of ireg * Int.int
+| Pmovq_ri of ireg * Int64.int
+| Pmov_rs of ireg * ident
+| Pmovl_rm of ireg * addrmode
+| Pmovq_rm of ireg * addrmode
+| Pmovl_mr of addrmode * ireg
+| Pmovq_mr of addrmode * ireg
+| Pmovsd_ff of freg * freg
+| Pmovsd_fi of freg * float
+| Pmovsd_fm of freg * addrmode
+| Pmovsd_mf of addrmode * freg
+| Pmovss_fi of freg * float32
+| Pmovss_fm of freg * addrmode
+| Pmovss_mf of addrmode * freg
+| Pfldl_m of addrmode
+| Pfstpl_m of addrmode
+| Pflds_m of addrmode
+| Pfstps_m of addrmode
+| Pmovb_mr of addrmode * ireg
+| Pmovw_mr of addrmode * ireg
+| Pmovzb_rr of ireg * ireg
+| Pmovzb_rm of ireg * addrmode
+| Pmovsb_rr of ireg * ireg
+| Pmovsb_rm of ireg * addrmode
+| Pmovzw_rr of ireg * ireg
+| Pmovzw_rm of ireg * addrmode
+| Pmovsw_rr of ireg * ireg
+| Pmovsw_rm of ireg * addrmode
+| Pmovzl_rr of ireg * ireg
+| Pmovsl_rr of ireg * ireg
+| Pmovls_rr of ireg
+| Pcvtsd2ss_ff of freg * freg
+| Pcvtss2sd_ff of freg * freg
+| Pcvttsd2si_rf of ireg * freg
+| Pcvtsi2sd_fr of freg * ireg
+| Pcvttss2si_rf of ireg * freg
+| Pcvtsi2ss_fr of freg * ireg
+| Pcvttsd2sl_rf of ireg * freg
+| Pcvtsl2sd_fr of freg * ireg
+| Pcvttss2sl_rf of ireg * freg
+| Pcvtsl2ss_fr of freg * ireg
+| Pleal of ireg * addrmode
+| Pleaq of ireg * addrmode
+| Pnegl of ireg
+| Pnegq of ireg
+| Paddl_ri of ireg * Int.int
+| Paddq_ri of ireg * Int64.int
+| Psubl_rr of ireg * ireg
+| Psubq_rr of ireg * ireg
+| Pimull_rr of ireg * ireg
+| Pimulq_rr of ireg * ireg
+| Pimull_ri of ireg * Int.int
+| Pimulq_ri of ireg * Int64.int
+| Pimull_r of ireg
+| Pimulq_r of ireg
+| Pmull_r of ireg
+| Pmulq_r of ireg
+| Pcltd
+| Pcqto
+| Pdivl of ireg
+| Pdivq of ireg
+| Pidivl of ireg
+| Pidivq of ireg
+| Pandl_rr of ireg * ireg
+| Pandq_rr of ireg * ireg
+| Pandl_ri of ireg * Int.int
+| Pandq_ri of ireg * Int64.int
+| Porl_rr of ireg * ireg
+| Porq_rr of ireg * ireg
+| Porl_ri of ireg * Int.int
+| Porq_ri of ireg * Int64.int
+| Pxorl_r of ireg
+| Pxorq_r of ireg
+| Pxorl_rr of ireg * ireg
+| Pxorq_rr of ireg * ireg
+| Pxorl_ri of ireg * Int.int
+| Pxorq_ri of ireg * Int64.int
+| Pnotl of ireg
+| Pnotq of ireg
+| Psall_rcl of ireg
+| Psalq_rcl of ireg
+| Psall_ri of ireg * Int.int
+| Psalq_ri of ireg * Int.int
+| Pshrl_rcl of ireg
+| Pshrq_rcl of ireg
+| Pshrl_ri of ireg * Int.int
+| Pshrq_ri of ireg * Int.int
+| Psarl_rcl of ireg
+| Psarq_rcl of ireg
+| Psarl_ri of ireg * Int.int
+| Psarq_ri of ireg * Int.int
+| Pshld_ri of ireg * ireg * Int.int
+| Prorl_ri of ireg * Int.int
+| Prorq_ri of ireg * Int.int
+| Pcmpl_rr of ireg * ireg
+| Pcmpq_rr of ireg * ireg
+| Pcmpl_ri of ireg * Int.int
+| Pcmpq_ri of ireg * Int64.int
+| Ptestl_rr of ireg * ireg
+| Ptestq_rr of ireg * ireg
+| Ptestl_ri of ireg * Int.int
+| Ptestq_ri of ireg * Int64.int
+| Pcmov of testcond * ireg * ireg
+| Psetcc of testcond * ireg
+| Paddd_ff of freg * freg
+| Psubd_ff of freg * freg
+| Pmuld_ff of freg * freg
+| Pdivd_ff of freg * freg
+| Pnegd of freg
+| Pabsd of freg
+| Pcomisd_ff of freg * freg
+| Pxorpd_f of freg
+| Padds_ff of freg * freg
+| Psubs_ff of freg * freg
+| Pmuls_ff of freg * freg
+| Pdivs_ff of freg * freg
+| Pnegs of freg
+| Pabss of freg
+| Pcomiss_ff of freg * freg
+| Pxorps_f of freg
+| Pjmp_l of label
+| Pjmp_s of ident * signature
+| Pjmp_r of ireg * signature
+| Pjcc of testcond * label
+| Pjcc2 of testcond * testcond * label
+| Pjmptbl of ireg * label list
+| Pcall_s of ident * signature
+| Pcall_r of ireg * signature
+| Pret
+| Pmov_rm_a of ireg * addrmode
+| Pmov_mr_a of addrmode * ireg
+| Pmovsd_fm_a of freg * addrmode
+| Pmovsd_mf_a of addrmode * freg
+| Plabel of label
+| Pallocframe of z * Ptrofs.int * Ptrofs.int
+| Pfreeframe of z * Ptrofs.int * Ptrofs.int
+| Pbuiltin of external_function * preg builtin_arg list * preg builtin_res
+| Padcl_ri of ireg * Int.int
+| Padcl_rr of ireg * ireg
+| Paddl_mi of addrmode * Int.int
+| Paddl_rr of ireg * ireg
+| Pbsfl of ireg * ireg
+| Pbsfq of ireg * ireg
+| Pbsrl of ireg * ireg
+| Pbsrq of ireg * ireg
+| Pbswap64 of ireg
+| Pbswap32 of ireg
+| Pbswap16 of ireg
+| Pcfi_adjust of Int.int
+| Pfmadd132 of freg * freg * freg
+| Pfmadd213 of freg * freg * freg
+| Pfmadd231 of freg * freg * freg
+| Pfmsub132 of freg * freg * freg
+| Pfmsub213 of freg * freg * freg
+| Pfmsub231 of freg * freg * freg
+| Pfnmadd132 of freg * freg * freg
+| Pfnmadd213 of freg * freg * freg
+| Pfnmadd231 of freg * freg * freg
+| Pfnmsub132 of freg * freg * freg
+| Pfnmsub213 of freg * freg * freg
+| Pfnmsub231 of freg * freg * freg
+| Pmaxsd of freg * freg
+| Pminsd of freg * freg
+| Pmovb_rm of ireg * addrmode
+| Pmovq_rf of ireg * freg
+| Pmovsq_mr of addrmode * freg
+| Pmovsq_rm of freg * addrmode
+| Pmovsb
+| Pmovsw
+| Pmovw_rm of ireg * addrmode
+| Pnop
+| Prep_movsl
+| Psbbl_rr of ireg * ireg
+| Psqrtsd of freg * freg
+| Psubl_ri of ireg * Int.int
+| Psubq_ri of ireg * Int64.int
+
+type code = instruction0 list
+
+type function0 = { fn_sig : signature; fn_code : code }
+
+(** val bytecode_signature : signature **)
+
+let bytecode_signature =
+  { sig_args = (Cons (Xptr, (Cons (Xint, (Cons (Xptr, (Cons (Xint,
+    Nil)))))))); sig_res = Xvoid; sig_cc = cc_default }
+
+(** val word_bytes : z **)
+
+let word_bytes =
+  Zpos (XO (XO (XO (XO (XO XH)))))
+
+(** val word_limb_bytes : z **)
+
+let word_limb_bytes =
+  Zpos (XO (XO XH))
+
+(** val word_limb_count : nat **)
+
+let word_limb_count =
+  S (S (S (S (S (S (S (S O)))))))
+
+(** val native_stack_limit_words : z **)
+
+let native_stack_limit_words =
+  Zpos (XO (XO (XO (XO (XO (XO (XO (XO (XO (XO XH))))))))))
+
+(** val frame_link_offset : z **)
+
+let frame_link_offset =
+  Z0
+
+(** val frame_ra_offset : z **)
+
+let frame_ra_offset =
+  Zpos (XO (XO (XO XH)))
+
+(** val frame_stack_base : z **)
+
+let frame_stack_base =
+  Zpos (XO (XO (XO (XO XH))))
+
+(** val frame_stack_bytes : z **)
+
+let frame_stack_bytes =
+  Z.mul native_stack_limit_words word_bytes
+
+(** val frame_size : z **)
+
+let frame_size =
+  Z.add frame_stack_base frame_stack_bytes
+
+(** val frame_link_ptrofs : Ptrofs.int **)
+
+let frame_link_ptrofs =
+  Ptrofs.repr frame_link_offset
+
+(** val frame_ra_ptrofs : Ptrofs.int **)
+
+let frame_ra_ptrofs =
+  Ptrofs.repr frame_ra_offset
+
+(** val arg_in : ireg **)
+
+let arg_in =
+  RDI
+
+(** val arg_insize : ireg **)
+
+let arg_insize =
+  RSI
+
+(** val arg_out : ireg **)
+
+let arg_out =
+  RDX
+
+(** val arg_outsize : ireg **)
+
+let arg_outsize =
+  RCX
+
+(** val stack_ptr_reg : ireg **)
+
+let stack_ptr_reg =
+  R8
+
+(** val tmp0 : ireg **)
+
+let tmp0 =
+  R9
+
+(** val tmp1 : ireg **)
+
+let tmp1 =
+  R10
+
+(** val as_int : z -> Int.int **)
+
+let as_int =
+  Int.repr
+
+(** val as_int64 : z -> Int64.int **)
+
+let as_int64 =
+  Int64.repr
+
+(** val reg_addr : ireg -> z -> addrmode **)
+
+let reg_addr base ofs =
+  Addrmode ((Some base), None, (Inl ofs))
+
+(** val pc_label : nat -> label **)
+
+let pc_label =
+  Coq_Pos.of_succ_nat
+
+(** val label_span : program -> nat **)
+
+let label_span p =
+  S (length p.program_bytes)
+
+(** val local_label : program -> nat -> nat -> nat -> label **)
+
+let local_label p tag pc slot =
+  Coq_Pos.of_succ_nat
+    (add
+      (add
+        (add (length p.program_bytes)
+          (mul (mul tag (label_span p)) (label_span p)))
+        (mul pc (label_span p)))
+      slot)
+
+(** val halt_label : program -> label **)
+
+let halt_label p =
+  local_label p (S O) O O
+
+(** val jump_zero_label : program -> nat -> label **)
+
+let jump_zero_label p pc =
+  local_label p (S (S O)) pc O
+
+(** val jump_case_label : program -> nat -> nat -> label **)
+
+let jump_case_label p pc case_index =
+  local_label p (S (S (S O))) pc case_index
+
+(** val limb_offset : nat -> z **)
+
+let limb_offset limb =
+  Z.mul word_limb_bytes (Z.of_nat limb)
+
+(** val internal_word_offset : nat -> nat -> z **)
+
+let internal_word_offset word_index limb =
+  Z.add (Z.mul word_bytes (Z.of_nat word_index)) (limb_offset limb)
+
+(** val external_word_offset : nat -> nat -> z **)
+
+let external_word_offset word_index limb =
+  Z.add (Z.mul word_bytes (Z.of_nat word_index))
+    (Z.mul word_limb_bytes
+      (Z.of_nat (sub (S (S (S (S (S (S (S O))))))) limb)))
+
+(** val frame_stack_end : z **)
+
+let frame_stack_end =
+  Z.add frame_stack_base frame_stack_bytes
+
+(** val word_limb : z -> nat -> z **)
+
+let word_limb value limb =
+  Z.coq_land
+    (Z.shiftr value
+      (Z.mul (Zpos (XO (XO (XO (XO (XO XH)))))) (Z.of_nat limb)))
+    (Z.ones (Zpos (XO (XO (XO (XO (XO XH)))))))
+
+(** val word_limb_int : z -> nat -> Int.int **)
+
+let word_limb_int value limb =
+  as_int (word_limb value limb)
+
+(** val all_limbs : nat list **)
+
+let all_limbs =
+  seq O word_limb_count
+
+(** val compile_limb_code : (nat -> code) -> nat list -> code **)
+
+let rec compile_limb_code f = function
+| Nil -> Nil
+| Cons (limb, rest) -> app (f limb) (compile_limb_code f rest)
+
+(** val jumpdest_pcs : program -> nat list **)
+
+let jumpdest_pcs p =
+  fold_right (fun i acc ->
+    match i.instr_opcode with
+    | OpJumpdest -> Cons (i.instr_pc, acc)
+    | _ -> acc) Nil p.program_code
+
+(** val init_stack_pointer : code **)
+
+let init_stack_pointer =
+  Cons ((Pleaq (stack_ptr_reg, (reg_addr RSP frame_stack_base))), Nil)
+
+(** val halt_if_stack_full : label -> code **)
+
+let halt_if_stack_full halt =
+  Cons ((Pleaq (tmp0, (reg_addr RSP frame_stack_end))), (Cons ((Pcmpq_rr
+    (stack_ptr_reg, tmp0)), (Cons ((Pjcc (Cond_ae, halt)), Nil)))))
+
+(** val halt_if_stack_below : z -> label -> code **)
+
+let halt_if_stack_below required_bytes halt =
+  Cons ((Pleaq (tmp0,
+    (reg_addr RSP (Z.add frame_stack_base required_bytes)))), (Cons
+    ((Pcmpq_rr (stack_ptr_reg, tmp0)), (Cons ((Pjcc (Cond_b, halt)), Nil)))))
+
+(** val halt_if_input_oob : nat -> label -> code **)
+
+let halt_if_input_oob index halt =
+  Cons ((Pcmpq_ri (arg_insize, (as_int64 (Z.of_nat index)))), (Cons ((Pjcc
+    (Cond_be, halt)), Nil)))
+
+(** val halt_if_output_oob : nat -> label -> code **)
+
+let halt_if_output_oob index halt =
+  Cons ((Pcmpq_ri (arg_outsize, (as_int64 (Z.of_nat index)))), (Cons ((Pjcc
+    (Cond_be, halt)), Nil)))
+
+(** val load_external_word : ireg -> nat -> ireg -> nat -> code **)
+
+let load_external_word src_base src_index dst_base dst_word_index =
+  compile_limb_code (fun limb -> Cons ((Pmovl_rm (tmp0,
+    (reg_addr src_base (external_word_offset src_index limb)))), (Cons
+    ((Pbswap32 tmp0), (Cons ((Pmovl_mr
+    ((reg_addr dst_base (internal_word_offset dst_word_index limb)), tmp0)),
+    Nil)))))) all_limbs
+
+(** val store_external_word_from_offset : ireg -> z -> ireg -> nat -> code **)
+
+let store_external_word_from_offset src_base src_ofs dst_base dst_index =
+  compile_limb_code (fun limb -> Cons ((Pmovl_rm (tmp0,
+    (reg_addr src_base (Z.add src_ofs (limb_offset limb))))), (Cons
+    ((Pbswap32 tmp0), (Cons ((Pmovl_mr
+    ((reg_addr dst_base (external_word_offset dst_index limb)), tmp0)),
+    Nil)))))) all_limbs
+
+(** val copy_internal_word_from_offset : ireg -> z -> ireg -> nat -> code **)
+
+let copy_internal_word_from_offset src_base src_ofs dst_base dst_word_index =
+  compile_limb_code (fun limb -> Cons ((Pmovl_rm (tmp0,
+    (reg_addr src_base (Z.add src_ofs (limb_offset limb))))), (Cons
+    ((Pmovl_mr
+    ((reg_addr dst_base (internal_word_offset dst_word_index limb)), tmp0)),
+    Nil)))) all_limbs
+
+(** val add_top_words : code **)
+
+let add_top_words =
+  app (Cons ((Pmovl_rm (tmp0,
+    (reg_addr stack_ptr_reg (Zneg (XO (XO (XO (XO (XO (XO XH)))))))))), (Cons
+    ((Pmovl_rm (tmp1,
+    (reg_addr stack_ptr_reg (Zneg (XO (XO (XO (XO (XO XH))))))))), (Cons
+    ((Paddl_rr (tmp0, tmp1)), (Cons ((Pmovl_mr
+    ((reg_addr stack_ptr_reg (Zneg (XO (XO (XO (XO (XO (XO XH)))))))),
+    tmp0)), Nil))))))))
+    (app
+      (compile_limb_code (fun limb -> Cons ((Pmovl_rm (tmp0,
+        (reg_addr stack_ptr_reg
+          (Z.add (Zneg (XO (XO (XO (XO (XO (XO XH)))))))
+            (limb_offset (S limb)))))),
+        (Cons ((Pmovl_rm (tmp1,
+        (reg_addr stack_ptr_reg
+          (Z.add (Zneg (XO (XO (XO (XO (XO XH)))))) (limb_offset (S limb)))))),
+        (Cons ((Padcl_rr (tmp0, tmp1)), (Cons ((Pmovl_mr
+        ((reg_addr stack_ptr_reg
+           (Z.add (Zneg (XO (XO (XO (XO (XO (XO XH)))))))
+             (limb_offset (S limb)))),
+        tmp0)), Nil)))))))) (seq O (S (S (S (S (S (S (S O)))))))))
+      (Cons ((Psubq_ri (stack_ptr_reg, (as_int64 word_bytes))), Nil)))
+
+(** val sub_top_words : code **)
+
+let sub_top_words =
+  app (Cons ((Pmovl_rm (tmp0,
+    (reg_addr stack_ptr_reg (Zneg (XO (XO (XO (XO (XO (XO XH)))))))))), (Cons
+    ((Pmovl_rm (tmp1,
+    (reg_addr stack_ptr_reg (Zneg (XO (XO (XO (XO (XO XH))))))))), (Cons
+    ((Psubl_rr (tmp0, tmp1)), (Cons ((Pmovl_mr
+    ((reg_addr stack_ptr_reg (Zneg (XO (XO (XO (XO (XO (XO XH)))))))),
+    tmp0)), Nil))))))))
+    (app
+      (compile_limb_code (fun limb -> Cons ((Pmovl_rm (tmp0,
+        (reg_addr stack_ptr_reg
+          (Z.add (Zneg (XO (XO (XO (XO (XO (XO XH)))))))
+            (limb_offset (S limb)))))),
+        (Cons ((Pmovl_rm (tmp1,
+        (reg_addr stack_ptr_reg
+          (Z.add (Zneg (XO (XO (XO (XO (XO XH)))))) (limb_offset (S limb)))))),
+        (Cons ((Psbbl_rr (tmp0, tmp1)), (Cons ((Pmovl_mr
+        ((reg_addr stack_ptr_reg
+           (Z.add (Zneg (XO (XO (XO (XO (XO (XO XH)))))))
+             (limb_offset (S limb)))),
+        tmp0)), Nil)))))))) (seq O (S (S (S (S (S (S (S O)))))))))
+      (Cons ((Psubq_ri (stack_ptr_reg, (as_int64 word_bytes))), Nil)))
+
+(** val zero_test_word_at : ireg -> z -> label -> code **)
+
+let zero_test_word_at base ofs on_zero =
+  app (Cons ((Pxorl_r tmp0), Nil))
+    (app
+      (compile_limb_code (fun limb -> Cons ((Pmovl_rm (tmp1,
+        (reg_addr base (Z.add ofs (limb_offset limb))))), (Cons ((Porl_rr
+        (tmp0, tmp1)), Nil)))) all_limbs)
+      (Cons ((Ptestl_rr (tmp0, tmp0)), (Cons ((Pjcc (Cond_e, on_zero)),
+      Nil)))))
+
+(** val compare_word_at_with : ireg -> z -> z -> label -> code **)
+
+let compare_word_at_with base ofs value on_mismatch =
+  compile_limb_code (fun limb -> Cons ((Pmovl_rm (tmp0,
+    (reg_addr base (Z.add ofs (limb_offset limb))))), (Cons ((Pcmpl_ri (tmp0,
+    (word_limb_int value limb))), (Cons ((Pjcc (Cond_ne, on_mismatch)),
+    Nil)))))) all_limbs
+
+(** val compile_jump_cases : program -> nat -> nat -> nat list -> code **)
+
+let rec compile_jump_cases p pc case_index = function
+| Nil -> Cons ((Pjmp_l (halt_label p)), Nil)
+| Cons (destination, rest) ->
+  let miss = jump_case_label p pc case_index in
+  app
+    (compare_word_at_with stack_ptr_reg word_bytes (Z.of_nat destination)
+      miss)
+    (app (Cons ((Pjmp_l (pc_label destination)), (Cons ((Plabel miss),
+      Nil)))) (compile_jump_cases p pc (S case_index) rest))
+
+(** val compile_push_from_input : program -> nat -> code **)
+
+let compile_push_from_input p index =
+  app (halt_if_input_oob index (halt_label p))
+    (app (halt_if_stack_full (halt_label p))
+      (app (load_external_word arg_in index stack_ptr_reg O) (Cons ((Paddq_ri
+        (stack_ptr_reg, (as_int64 word_bytes))), Nil))))
+
+(** val compile_store_to_output : program -> nat -> code **)
+
+let compile_store_to_output p index =
+  app (halt_if_output_oob index (halt_label p))
+    (app (halt_if_stack_below word_bytes (halt_label p))
+      (app
+        (store_external_word_from_offset stack_ptr_reg (Z.opp word_bytes)
+          arg_out index)
+        (Cons ((Psubq_ri (stack_ptr_reg, (as_int64 word_bytes))), Nil))))
+
+(** val compile_dup : program -> code **)
+
+let compile_dup p =
+  app (halt_if_stack_below word_bytes (halt_label p))
+    (app (halt_if_stack_full (halt_label p))
+      (app
+        (copy_internal_word_from_offset stack_ptr_reg (Z.opp word_bytes)
+          stack_ptr_reg O)
+        (Cons ((Paddq_ri (stack_ptr_reg, (as_int64 word_bytes))), Nil))))
+
+(** val compile_jumpi : program -> nat -> code **)
+
+let compile_jumpi p pc =
+  app (halt_if_stack_below (Z.mul (Zpos (XO XH)) word_bytes) (halt_label p))
+    (app
+      (zero_test_word_at stack_ptr_reg (Zneg (XO (XO (XO (XO (XO (XO
+        XH))))))) (jump_zero_label p pc))
+      (app (Cons ((Psubq_ri (stack_ptr_reg,
+        (as_int64 (Z.mul (Zpos (XO XH)) word_bytes)))), Nil))
+        (app (compile_jump_cases p pc O (jumpdest_pcs p)) (Cons ((Plabel
+          (jump_zero_label p pc)), (Cons ((Psubq_ri (stack_ptr_reg,
+          (as_int64 (Z.mul (Zpos (XO XH)) word_bytes)))), Nil)))))))
+
+(** val transl_instruction : program -> instruction -> code **)
+
+let transl_instruction p i =
+  match i.instr_opcode with
+  | OpStop -> Cons ((Pjmp_l (halt_label p)), Nil)
+  | OpLoad index -> compile_push_from_input p index
+  | OpStore index -> compile_store_to_output p index
+  | OpPop ->
+    app (halt_if_stack_below word_bytes (halt_label p)) (Cons ((Psubq_ri
+      (stack_ptr_reg, (as_int64 word_bytes))), Nil))
+  | OpAdd ->
+    app
+      (halt_if_stack_below (Z.mul (Zpos (XO XH)) word_bytes) (halt_label p))
+      add_top_words
+  | OpSub ->
+    app
+      (halt_if_stack_below (Z.mul (Zpos (XO XH)) word_bytes) (halt_label p))
+      sub_top_words
+  | OpDup -> compile_dup p
+  | OpJumpdest -> Nil
+  | OpJumpi -> compile_jumpi p i.instr_pc
+
+(** val transl_labeled_instruction : program -> instruction -> code **)
+
+let transl_labeled_instruction p i =
+  Cons ((Plabel (pc_label i.instr_pc)), (transl_instruction p i))
+
+(** val transl_code : program -> instruction list -> code **)
+
+let rec transl_code p = function
+| Nil -> Nil
+| Cons (i, rest) -> app (transl_labeled_instruction p i) (transl_code p rest)
+
+(** val transl_program_code : program -> code **)
+
+let transl_program_code p =
+  app (Cons ((Pallocframe (frame_size, frame_ra_ptrofs, frame_link_ptrofs)),
+    Nil))
+    (app init_stack_pointer
+      (app (transl_code p p.program_code) (Cons ((Plabel (halt_label p)),
+        (Cons ((Pfreeframe (frame_size, frame_ra_ptrofs, frame_link_ptrofs)),
+        (Cons (Pret, Nil))))))))
+
+(** val transl_program : program -> function0 **)
+
+let transl_program p =
+  { fn_sig = bytecode_signature; fn_code = (transl_program_code p) }
+
+(** val transl_bytes : Byte.t list -> function0 parse_result **)
+
+let transl_bytes bytes =
+  match parse bytes with
+  | Parsed p -> Parsed (transl_program p)
+  | Rejected error -> Rejected error
