tools/tmp/f.s
@@ -1,0 +1,142 @@
+	.text
+	.globl _f
+_f:
+	subq	$32776, %rsp
+	leaq	32784(%rsp), %rax
+	movq	%rax, 0(%rsp)
+	leaq	16(%rsp), %r8
+.L1:
+	cmpq	$0, %rsi
+	jbe	.L90
+	leaq	32784(%rsp), %r9
+	cmpq	%r9, %r8
+	jae	.L90
+	movl	28(%rdi), %r9d
+	bswap	%r9d
+	movl	%r9d, (%r8)
+	movl	24(%rdi), %r9d
+	bswap	%r9d
+	movl	%r9d, 4(%r8)
+	movl	20(%rdi), %r9d
+	bswap	%r9d
+	movl	%r9d, 8(%r8)
+	movl	16(%rdi), %r9d
+	bswap	%r9d
+	movl	%r9d, 12(%r8)
+	movl	12(%rdi), %r9d
+	bswap	%r9d
+	movl	%r9d, 16(%r8)
+	movl	8(%rdi), %r9d
+	bswap	%r9d
+	movl	%r9d, 20(%r8)
+	movl	4(%rdi), %r9d
+	bswap	%r9d
+	movl	%r9d, 24(%r8)
+	movl	(%rdi), %r9d
+	bswap	%r9d
+	movl	%r9d, 28(%r8)
+	addq	$32, %r8
+.L3:
+	cmpq	$1, %rsi
+	jbe	.L90
+	leaq	32784(%rsp), %r9
+	cmpq	%r9, %r8
+	jae	.L90
+	movl	60(%rdi), %r9d
+	bswap	%r9d
+	movl	%r9d, (%r8)
+	movl	56(%rdi), %r9d
+	bswap	%r9d
+	movl	%r9d, 4(%r8)
+	movl	52(%rdi), %r9d
+	bswap	%r9d
+	movl	%r9d, 8(%r8)
+	movl	48(%rdi), %r9d
+	bswap	%r9d
+	movl	%r9d, 12(%r8)
+	movl	44(%rdi), %r9d
+	bswap	%r9d
+	movl	%r9d, 16(%r8)
+	movl	40(%rdi), %r9d
+	bswap	%r9d
+	movl	%r9d, 20(%r8)
+	movl	36(%rdi), %r9d
+	bswap	%r9d
+	movl	%r9d, 24(%r8)
+	movl	32(%rdi), %r9d
+	bswap	%r9d
+	movl	%r9d, 28(%r8)
+	addq	$32, %r8
+.L5:
+	leaq	80(%rsp), %r9
+	cmpq	%r9, %r8
+	jb	.L90
+	movl	-64(%r8), %r9d
+	movl	-32(%r8), %r10d
+	addl	%r10d, %r9d
+	movl	%r9d, -64(%r8)
+	movl	-60(%r8), %r9d
+	movl	-28(%r8), %r10d
+	adcl	%r10d, %r9d
+	movl	%r9d, -60(%r8)
+	movl	-56(%r8), %r9d
+	movl	-24(%r8), %r10d
+	adcl	%r10d, %r9d
+	movl	%r9d, -56(%r8)
+	movl	-52(%r8), %r9d
+	movl	-20(%r8), %r10d
+	adcl	%r10d, %r9d
+	movl	%r9d, -52(%r8)
+	movl	-48(%r8), %r9d
+	movl	-16(%r8), %r10d
+	adcl	%r10d, %r9d
+	movl	%r9d, -48(%r8)
+	movl	-44(%r8), %r9d
+	movl	-12(%r8), %r10d
+	adcl	%r10d, %r9d
+	movl	%r9d, -44(%r8)
+	movl	-40(%r8), %r9d
+	movl	-8(%r8), %r10d
+	adcl	%r10d, %r9d
+	movl	%r9d, -40(%r8)
+	movl	-36(%r8), %r9d
+	movl	-4(%r8), %r10d
+	adcl	%r10d, %r9d
+	movl	%r9d, -36(%r8)
+	subq	$32, %r8
+.L6:
+	cmpq	$0, %rcx
+	jbe	.L90
+	leaq	48(%rsp), %r9
+	cmpq	%r9, %r8
+	jb	.L90
+	movl	-32(%r8), %r9d
+	bswap	%r9d
+	movl	%r9d, 28(%rdx)
+	movl	-28(%r8), %r9d
+	bswap	%r9d
+	movl	%r9d, 24(%rdx)
+	movl	-24(%r8), %r9d
+	bswap	%r9d
+	movl	%r9d, 20(%rdx)
+	movl	-20(%r8), %r9d
+	bswap	%r9d
+	movl	%r9d, 16(%rdx)
+	movl	-16(%r8), %r9d
+	bswap	%r9d
+	movl	%r9d, 12(%rdx)
+	movl	-12(%r8), %r9d
+	bswap	%r9d
+	movl	%r9d, 8(%rdx)
+	movl	-8(%r8), %r9d
+	bswap	%r9d
+	movl	%r9d, 4(%rdx)
+	movl	-4(%r8), %r9d
+	bswap	%r9d
+	movl	%r9d, (%rdx)
+	subq	$32, %r8
+.L8:
+	jmp	.L90
+.L90:
+	addq	$32776, %rsp
+	ret
